Trident/Target/Dialect.lean
@@ -140,4 +140,6 @@ def TritonOp.arity : TritonOp → Nat
   | .storef => 2
   | .constant_tensorf _ _ => 0
 
+
+
 end Trident
